type lifting
Signed-off-by: Shaobo He <shaobohe@amazon.com>

cedar-lean/Cedar/Validation/TypedExpr.lean
@@ -153,31 +153,30 @@ def TypedExpr.toExpr : TypedExpr → Expr
       omega
     e.toExpr)
 
-def TypedExpr.liftBoolType : TypedExpr → TypedExpr
-  | .lit p ty => .lit p ty.liftBoolType
-  | .var v ty =>  .var v ty.liftBoolType
-  | .ite cond thenExpr elseExpr ty => .ite cond.liftBoolType thenExpr.liftBoolType elseExpr.liftBoolType ty.liftBoolType
-  | .and a b ty => .and a.liftBoolType b.liftBoolType ty.liftBoolType
-  | .or a b ty => .or a.liftBoolType b.liftBoolType ty.liftBoolType
-  | .unaryApp op expr ty => .unaryApp op expr.liftBoolType ty.liftBoolType
-  | .binaryApp op a b ty => .binaryApp op a.liftBoolType b.liftBoolType ty.liftBoolType
-  | .getAttr expr attr ty => .getAttr expr.liftBoolType attr ty.liftBoolType
-  | .hasAttr expr attr ty => .hasAttr expr.liftBoolType attr ty.liftBoolType
+def TypedExpr.liftBoolTypes : TypedExpr → TypedExpr
+  | .lit p ty => .lit p ty.liftBoolTypes
+  | .var v ty =>  .var v ty.liftBoolTypes
+  | .ite cond thenExpr elseExpr ty => .ite cond.liftBoolTypes thenExpr.liftBoolTypes elseExpr.liftBoolTypes ty.liftBoolTypes
+  | .and a b ty => .and a.liftBoolTypes b.liftBoolTypes ty.liftBoolTypes
+  | .or a b ty => .or a.liftBoolTypes b.liftBoolTypes ty.liftBoolTypes
+  | .unaryApp op expr ty => .unaryApp op expr.liftBoolTypes ty.liftBoolTypes
+  | .binaryApp op a b ty => .binaryApp op a.liftBoolTypes b.liftBoolTypes ty.liftBoolTypes
+  | .getAttr expr attr ty => .getAttr expr.liftBoolTypes attr ty.liftBoolTypes
+  | .hasAttr expr attr ty => .hasAttr expr.liftBoolTypes attr ty.liftBoolTypes
   | .set ls ty => .set (ls.map₁ (λ ⟨e, h₁⟩  =>
     have _ : sizeOf e < 1 + sizeOf ls + sizeOf ty := by
       have := List.sizeOf_lt_of_mem h₁
       omega
-    e.liftBoolType)) ty.liftBoolType
-  | .record ls ty => .record (ls.map₁ (λ ⟨(a, e), h₁⟩  =>
+    e.liftBoolTypes)) ty.liftBoolTypes
+  | .record ls ty => .record (ls.attach₂.map (λ ⟨(a, e), h₁⟩  =>
     have _ : sizeOf e < 1 + sizeOf ls + sizeOf ty := by
-      have := Map.sizeOf_lt_of_value h₁
-      simp only [Map.mk.sizeOf_spec] at this
+      simp only at h₁
       omega
-    (a, e.liftBoolType))) ty.liftBoolType
+    (a, e.liftBoolTypes))) ty.liftBoolTypes
   | .call xfn args ty => .call xfn (args.map₁ (λ ⟨e, h₁⟩  =>
     have _ : sizeOf e < 1 + sizeOf args + sizeOf ty := by
       have := List.sizeOf_lt_of_mem h₁
       omega
-    e.liftBoolType)) ty.liftBoolType
+    e.liftBoolTypes)) ty.liftBoolTypes
 
 end Cedar.Validation
